

Dr Li Ma (Spring Term)

Velocity Potential  $\phi$  and Stream Function  $\psi$ 

In Cartesian co-ordinates  $u = \frac{\partial \phi}{\partial x} = \frac{\partial \psi}{\partial z}$  ,  $w = \frac{\partial \phi}{\partial z} = -\frac{\partial \psi}{\partial x}$

In Polar Co-ordinates  $u_r = \frac{\partial \phi}{\partial r} = \frac{1}{r} \frac{\partial \psi}{\partial \theta}$  ,  $u_\theta = \frac{1}{r} \frac{\partial \phi}{\partial \theta} = -\frac{\partial \psi}{\partial r}$

Mass Continuity for 2-D flow

$$\frac{\partial u}{\partial x} + \frac{\partial w}{\partial z} = 0$$

Vorticity in a 2-D flow

$$\Omega = \frac{\partial w}{\partial x} - \frac{\partial u}{\partial z}$$

Equations of Motion for a 2-D flow

$$\frac{\partial u}{\partial t} + u \frac{\partial u}{\partial x} + w \frac{\partial u}{\partial z} = -\frac{1}{\rho} \frac{\partial P}{\partial x} \quad ; \quad \frac{\partial w}{\partial t} + u \frac{\partial w}{\partial x} + w \frac{\partial w}{\partial z} = -\frac{1}{\rho} \frac{\partial P}{\partial z} - g$$

Unsteady Bernoulli's Equation

$$\rho \frac{\partial \phi}{\partial t} + P + \rho g z + \rho \left( \frac{u^2 + w^2}{2} \right) = \text{constant}$$

Small Amplitude Wave Theory

$\eta = a \sin(\omega t - kx)$   $u = a \omega e^{kz} \sin(\omega t - kx)$ ;  $w = a \omega e^{kz} \cos(\omega t - kx)$  if deep water.

$$u = \frac{a \omega \cosh k(z+d)}{\sinh(kd)} \sin(\omega t - kx) \quad ; \quad w = \frac{a \omega \sinh k(z+d)}{\sinh(kd)} \cos(\omega t - kx) ;$$

$$p = \frac{\rho g a \cosh k(z+d)}{\cosh(kd)} \sin(\omega t - kx) - \rho g z$$

$$c = \frac{\omega}{k} = \left[ \frac{g}{k} \tanh(kd) \right]^{1/2}$$

$$\frac{c_g}{c} = \frac{1}{2} \left[ 1 + \frac{2kd}{\sinh(2kd)} \right]$$

**Variation of Wave Height in Shallow Water**

$$\frac{a^2}{k} \left[ 1 + \frac{2kd}{\sinh(2kd)} \right] = \text{constant}$$

**Energy in one wavelength**

$$PE_{WAVES} = KE_{WAVES} = \rho g \frac{a^2 \lambda}{4}$$

Instead of this I remember:  
 $E = \frac{\rho g a^2}{2} [\text{Jm}^{-1}]$  ← more flexible:  $[\text{Jm}^{-2}][\text{m}][\text{ms}^{-1}]$   
 can find Power =  $E \times \lambda \times c_g$  and etc.

**Potential flow about a vertical cylinder**

$$\phi = u \left( r + \frac{D^2}{4r} \right) \cos \theta \quad \text{for} \quad r \geq \frac{D}{2}$$

**Morison's Equation**

$$F = C_D \frac{1}{2} \rho u |u| D + C_M \rho \frac{\pi D^2}{4} \frac{du}{dt} \quad (\text{N/m})$$

**Useful identities**

$$\cosh^2(\theta) = \frac{1}{2} [\cosh(2\theta) + 1]$$

$$\sinh(\theta) = \frac{(e^\theta - e^{-\theta})}{2}, \cosh(\theta) = \frac{(e^\theta + e^{-\theta})}{2}$$

**Dr H Burrridge (Autumn Term)****Real Fluids**

Shear Stress  $\tau = \mu \frac{\partial u}{\partial y}$

Viscosity  $\nu = \frac{\mu}{\rho}$

	$\rho$ [kg/m <sup>3</sup> ]	$\nu$ [m <sup>2</sup> /s]
Air	1.2	$1.5 \cdot 10^{-5}$
Water	1000	$1.0 \cdot 10^{-6}$
Oil	910	$4 \cdot 10^{-4}$

**Navier Stokes**

$$\rho \left( \frac{\partial u}{\partial t} + u \frac{\partial u}{\partial x} + v \frac{\partial u}{\partial y} + w \frac{\partial u}{\partial z} \right) = -\frac{\partial P}{\partial x} + \rho g_x + \mu \left( \frac{\partial^2 u}{\partial x^2} + \frac{\partial^2 u}{\partial y^2} + \frac{\partial^2 u}{\partial z^2} \right)$$

$$\rho \left( \frac{\partial v}{\partial t} + u \frac{\partial v}{\partial x} + v \frac{\partial v}{\partial y} + w \frac{\partial v}{\partial z} \right) = -\frac{\partial P}{\partial y} + \rho g_y + \mu \left( \frac{\partial^2 v}{\partial x^2} + \frac{\partial^2 v}{\partial y^2} + \frac{\partial^2 v}{\partial z^2} \right)$$

$$\rho \left( \frac{\partial w}{\partial t} + u \frac{\partial w}{\partial x} + v \frac{\partial w}{\partial y} + w \frac{\partial w}{\partial z} \right) = -\frac{\partial P}{\partial z} + \rho g_z + \mu \left( \frac{\partial^2 w}{\partial x^2} + \frac{\partial^2 w}{\partial y^2} + \frac{\partial^2 w}{\partial z^2} \right)$$

**Notation:**  $\bar{u} = \bar{u}(x) = \frac{1}{T} \int_0^T u(x) dt$ , and  $U = \frac{1}{A} \int_0^A \bar{u}(x) dA$ , i.e.  $Q = U A$ .

$$dA = 2\pi r dr$$

Laminar (steady) flow between two very large parallel plates

$$u_{\max} = \frac{-B^2}{2\mu} \frac{d(p + \rho g \xi)}{dx}$$

$$u(y) = u_{\max} \left[ 1 - \left( \frac{y}{B} \right)^2 \right]$$

The drag force on a sphere in laminar (steady) flow is:

$$F_s = 3\pi \mu u D$$

Reynolds number:

$$\text{Re} = \frac{UL}{\nu}$$

## Steady Pipe Flow

$$\frac{p_1}{\rho g} + z_1 + \frac{U_1^2}{2g} + H_{\text{pump}} = \frac{p_2}{\rho g} + z_2 + \frac{U_2^2}{2g} + h_f + h_L$$

$$h_f = \frac{\tau_0 PL}{\rho g A} \quad (\tau_0 \text{ and } h_f \text{ interchangeable})$$

$$h_f = f \frac{L}{D} \frac{U^2}{2g}$$

$$(\tau_0 \text{ and } f \text{ or } U \text{ interchangeable}) \quad \tau_0 = \frac{f}{8} \rho U^2$$

$$f\left(\text{Re}, \frac{k_s}{D}\right)$$

first three rows are general eqn. that can be used for any pipe flow!

$$f = \frac{64}{\text{Re}} \quad \text{Re} < 2300$$

$$h_L = \xi \frac{U^2}{2g}$$

$$R_H = 4D$$

$$\frac{1}{f^{1/2}} = -2 \log_{10} \left[ \frac{k_s/D}{3.71} + \frac{2.51}{\text{Re} f^{1/2}} \right]$$

generally for any Re.

$$\left\{ R_H = \frac{A}{P} \quad \begin{array}{l} k_s/D = 0 \\ \text{if smooth} \end{array} \quad \begin{array}{l} \text{can get rid of this term if} \\ \text{Re very large. } (10^7) \end{array} \right.$$

$$u(r) = -\frac{1}{4\mu} \frac{dp}{dx} (R^2 - r^2) \quad \text{laminar } u(r) \text{ and } z(r)$$

$$\tau(r) = \mu \frac{du}{dr} = \frac{1}{2} \frac{dp}{dx} r$$

$$\frac{u_{\max} - \bar{u}(y)}{u_*} = -\frac{1}{\kappa} \ln \frac{y}{R} \quad \text{velocity defect law} \quad (3)$$

$$\kappa = 0.4$$

then to find  $\tau_0$

$$u_* = \sqrt{\tau_0 / \rho}$$

$$\frac{\bar{u}(y)}{u_*} = \frac{1}{\kappa} \ln \frac{y}{k_s} + 8.5 \quad \text{law of the wall} \quad (2)$$

$$\tau_0 = \rho u_*^2 = \frac{f}{8} \rho U^2$$

$$U = u_{\max} - \frac{3}{2} \frac{u_*}{\kappa} \quad \text{velocity defect law}$$

used to find  $u_p$

$$\frac{\bar{u}(y)}{u_*} = \frac{y}{\nu / u_*} \quad \text{viscous sub layer} \quad (1)$$

$$-\frac{\rho \bar{u}' v'}{\tau_0} = -\frac{\rho \bar{u}' v'}{\rho u_*^2} \approx 1 - \frac{y}{R}$$

$$u_* = \sqrt{\frac{f}{8}} U$$

## Pipe Systems

$$h_f + h_L = \left( f \frac{L}{D} + \sum_j \xi_j \right) \frac{Q^2}{2gA^2} = KQ^2$$

$$K = \frac{8}{g\pi^2 D^4} \left( f \frac{L}{D} + \sum_j \xi_j \right) \approx \frac{8fL}{g\pi^2 D^5}$$

$$f \approx \left[ \log_{10} \left( \frac{k_s/D}{3.71} \right)^{-2} \right]^{-2}$$

## Gradually-Variied Open Channel Flow

Bed Slope

$$S_0 = -\frac{dZ}{dx} \quad \tau_0 = \frac{f}{8} \rho U^2$$

$$\tau_0 = \rho g R S$$

Froude number:

$$Fr = \frac{U}{(gh)^{1/2}}$$

this h is not  $h_n$ ,  $h_c$  or current h!It's  $h_m$  (mean depth)where  $h_m = \frac{A}{W}$  ← cross sectional area of flow  
← width at surface.

Friction Factors

$$U = \frac{Q}{A} = \left( \frac{8g}{f} \right)^{1/2} R^{1/2} S^{1/2}$$

S = So if uniform

S = Sf if used in GVF

$$U = CR^{1/2} S^{1/2}$$

$$U = \frac{1}{n} R^{2/3} S^{1/2}$$

$$\frac{1}{f^{1/2}} = -2 \log_{10} \left( \frac{2.51}{Re f^{1/2}} + \frac{k_s / (4R)}{3.71} \right) \approx -2 \log_{10} \left( \frac{k_s / R}{14.84} \right)$$

$$f = \frac{8g}{C^2}$$

$$f = 8gn^2 / R^{1/3}$$

Specific Energy / Momentum

with respect to channel bed!

$$E(h) = h + \frac{q^2}{2gh^2} \quad J(h) = \frac{1}{2} \rho g h^2 + \frac{\rho q^2}{h}$$

no elevation head!

no weight component!

$$Fr = \frac{Q/A}{\sqrt{gA/b}}$$

Normal and Critical Depth

$$h_c = \left( \frac{q^2}{g} \right)^{1/3}$$

note that q is  $Q/w$ 

- valid for ANY rectangular channel.

If not rectangular channel:  $Fr = 1$   
(to find  $h_c$ )

$$\frac{U}{\sqrt{gh_m}} = 1 \text{ where } h_m = \frac{A}{w}$$

top width  
w

$$F(h_n) = 0 = \frac{Q}{A} - \left( \frac{8g}{f} \right)^{1/2} \left( \frac{A}{P} \right)^{1/2} S^{1/2}$$

used to find  $h_n$   
given Q

→ any channel (rectangular or not)

$$h_n = \left( \frac{fq^2}{8gS_0} \right)^{1/3}$$

used to find  $h_n$   
given Q

→ valid for ONLY wide rectangular channel.

S = So (cause uniform flow!)

Gradually Varied Flow

$$\frac{d\eta}{dx} = \frac{Q^2}{gA^3} \frac{dA}{dx} - \frac{fQ^2}{8gA^2R}$$

$$\frac{dh}{dx} = S_0 \frac{1 - (h_n/h)^3}{1 - (h_c/h)^3}$$

only valid for  
wide rectangular  
channel

$$\frac{S_0}{h_n} (x_2 - x_1) = (\gamma_2 - \gamma_1) - \left[ 1 - \left( \frac{h_c}{h_n} \right)^3 \right] (\Phi(\gamma_2) - \Phi(\gamma_1))$$

aim: to find  $x_2$ 

$$x_2 = x_1 + \frac{h_n}{S_0} \left\{ (\gamma_2 - \gamma_1) - \left[ 1 - \left( \frac{h_c}{h_n} \right)^3 \right] (\Phi(\gamma_2) - \Phi(\gamma_1)) \right\}$$

$$\Phi(\gamma) = \frac{1}{6} \ln \frac{\gamma^2 + \gamma + 1}{(\gamma - 1)^2} + \frac{1}{\sqrt{3}} \arctan \frac{2\gamma + 1}{\sqrt{3}}$$

$$\gamma \equiv \frac{h}{h_n}$$

$$\Phi(0.2) = 0.5027$$

$$\Phi(1.2) = 1.3867$$



